fixed proof in instr_dsstate_networking_common_invariants.dfy Delete a dumdd

dafny/ver/L1/distr_system_spec/adversary.dfy
@@ -22,20 +22,24 @@ module L1_Adversary
         && |a.byz| <= f(|validators([configuration.genesisBlock])|)
     }    
 
+    predicate isHonestByConfig(c: Configuration, a: Adversary, address: Address) {
+        address in (seqToSet(c.nodes) - a.byz)
+    }
+
     predicate AdvPrepare(preparePayload: SignedPrepare, c: Configuration, messagesReceived: set<QbftMessage>, a: Adversary) {
         || preparePayload in signedPreparePayloads(messagesReceived)
-        || !(recoverSignedPrepareAuthor(preparePayload) in seqToSet(c.nodes) - a.byz)
+        || !isHonestByConfig(c, a, recoverSignedPrepareAuthor(preparePayload))
     }
 
     predicate AdvBlock(b: Block, c: Configuration, messagesReceived: set<QbftMessage>, a: Adversary) {
         forall cs | cs in b.header.commitSeals ::
             || (cs in getCommitSeals(messagesReceived))
-            || !(recoverSignedHashAuthor(hashBlockForCommitSeal(b),cs) in seqToSet(c.nodes) - a.byz)
+            || (forall block:Block :: !isHonestByConfig(c, a, recoverSignedHashAuthor(hashBlockForCommitSeal(block),cs)))
     }
 
     predicate AdvRoundChange(m: SignedRoundChange, c: Configuration, messagesReceived: set<QbftMessage>, a: Adversary) {
         || m in signedRoundChangePayloads(messagesReceived)
-        || !(recoverSignedRoundChangeAuthor(m) in seqToSet(c.nodes) - a.byz) 
+        || !isHonestByConfig(c, a, recoverSignedRoundChangeAuthor(m)) 
     }
 
     
@@ -56,7 +60,7 @@ module L1_Adversary
                             && m.message.Proposal?
                             && (
                                 || m.message.proposalPayload in signedProposalPayloads(messagesReceived)
-                                || !(recoverSignedProposalAuthor(m.message.proposalPayload) in seqToSet(c.nodes) - a.byz)
+                                || !isHonestByConfig(c, a, recoverSignedProposalAuthor(m.message.proposalPayload))
                             )
                             && AdvBlock(m.message.proposedBlock, c, messagesReceived, a)
                             && (forall m' | m' in m.message.proposalJustification ::
@@ -83,14 +87,12 @@ module L1_Adversary
                         )
                         || (
                             && m.message.Commit?
-                            && !(recoverSignature(m.message) in seqToSet(c.nodes) - a.byz)
+                            && !isHonestByConfig(c, a, recoverSignature(m.message))
                             &&  var uPayload := m.message.commitPayload.unsignedPayload;
                                 var cs := uPayload.commitSeal;
                             && (
                                 || (cs in getCommitSeals(messagesReceived))
-                                || (forall b :: !(recoverSignedHashAuthor(hashBlockForCommitSeal(b), cs) in seqToSet(c.nodes) - a.byz))
-                                // not sure whether this is implementable (by public key cryptography)
-                            )
+                                || (forall b :: !isHonestByConfig(c, a, recoverSignedHashAuthor(hashBlockForCommitSeal(b), cs)))                            )
                         )                                        
                         || (
                             && m.message.NewBlock?
