test/test_helpers.dfy
@@ -10,46 +10,281 @@ import opened L1_Theorems
 import opened L1_TheoremsDefs
 import opened L1_AuxiliaryFunctionsAndLemmas
 
-// proposer 0,1,2,3
-function b1(): Block
-{
-    var b1 := Block(BlockHeader(0,0,{0},0,0), "the first proposal", ["trans1s"]);
-    b1
-}
-function b2(): Block
-{
-    var b2 := Block(BlockHeader(1,1,{0},1,3), "the second proposal", ["trans2s", "dummy transactions"]);
-    b2
-}
-function b3(): Block
-{
-    var b3 := Block(BlockHeader(2,2,{0},2,5), "the third proposal", ["trans3s"]);
-    b3
-}
 function genesisBlock(): Block
 {
     var header := BlockHeader(1, 0, {}, 0, 0);
-    Block(header, "", [])
+    Block(header, 0, [])
 }
-function c(): Configuration
+
+function config(): Configuration
 {
     Configuration([0,1,2,3], genesisBlock(), 0)
 }
-function BasicState(): DSState
+function env(): Network
 {
-    var env := Network([0,1,2,3], multiset{}, 0, multiset{});
-    var config := c();
-    DSState(config, env, map[], Adversary({}, {}))
+    // nodes, messagesSentYetToBeReceived, time, allMessagesSent
+    Network([0,1,2,3], multiset{}, 0, multiset{})
 }
-function StateGeneratorNoAdversary(blockchain0: Blockchain, blockchain1: Blockchain, blockchain2: Blockchain, blockchain3: Blockchain): DSState
+function adv(): Adversary
 {
-    var n0 := NodeState(blockchain0, 0, 0, 0, c(), {}, None, None, None, 0);
-    var n1 := NodeState(blockchain1, 0, 0, 1, c(), {}, None, None, None, 0);
-    var n2 := NodeState(blockchain2, 0, 0, 2, c(), {}, None, None, None, 0);
-    var n3 := NodeState(blockchain3, 0, 0, 3, c(), {}, None, None, None, 0);
-
-    var nodes := map[0 := n0, 1 := n1, 2 := n2, 3:= n3];
-    BasicState().(nodes := nodes)
+    Adversary({}, {1})
+}
+function s0(): DSState
+{
+    DSState(config(), env(), map[
+                // blockchain, round, localTime, id, configuration, messagesReceived, proposalAcceptedForCurrentRound, lastPreparedBlock, lastPreparedRound, timeLastRoundStart
+                0 := NodeState([genesisBlock()], 0, 0, 0, config(), {}, None, None, None, 0),
+                1 := NodeState([genesisBlock()], 0, 0, 1, config(), {}, None, None, None, 0),
+                2 := NodeState([genesisBlock()], 0, 0, 2, config(), {}, None, None, None, 0),
+                3 := NodeState([genesisBlock()], 0, 0, 3, config(), {}, None, None, None, 0)
+            ], adv())
 }
 
+function signedBlock(i:nat): Block
+{
+    // proposer, roundNumber, commitSeals, height, timestamp
+    var block1 := Block(BlockHeader(0, 0, {}, 1, 0), i, []); // a random block with empty commit seals
+    var commitSeals1 := {signHash(hashBlockForCommitSeal(block1), 1), signHash(hashBlockForCommitSeal(block1), 2), signHash(hashBlockForCommitSeal(block1), 3)}; // constructing valid commit seals from a quorum of honest nodes
+    block1.(header := block1.header.(commitSeals := commitSeals1)) // put the commit seals into the block
+}
+function proposalPayload(i:nat): SignedProposal
+{
+    signProposal(UnsignedProposal(0,0,digest(signedBlock(i))),0)
+}
+function proposal(i:nat): QbftMessageWithRecipient
+{
+    QbftMessageWithRecipient(Proposal(proposalPayload(i), signedBlock(i), {}, {}), 0)
+}
+function currentWithNewMessagesReceived1(): NodeState
+{
+    NodeState([genesisBlock()], 0, 1, 0, config(), {}, None, None, None, 0)
+}
+function outProposal1(i:nat): set<QbftMessageWithRecipient>
+{
+    Multicast(
+            [0,1,2,3],
+            proposal(i).message
+        )
+}
+function intermediateState1_1(): NodeState
+{
+    currentWithNewMessagesReceived1().(
+        messagesReceived := {proposal(1).message}
+    )
+}
+function intermediateState1_2(): NodeState
+{
+    intermediateState1_1().(
+        messagesReceived := intermediateState1_1().messagesReceived + {proposal(2).message}
+    )
+}
+function prepare1(): QbftMessage
+{
+    Prepare(
+            signPrepare(
+                UnsignedPrepare(
+                    1,
+                    0,
+                    digest(signedBlock(1))),
+                0
+                )
+        )
+}
+function outPrepare1(): set<QbftMessageWithRecipient>
+{
+    Multicast(
+                [0,1,2,3],
+                prepare1()
+            )
+}
+function finalState1(): NodeState
+{
+    intermediateState1_2().(
+        proposalAcceptedForCurrentRound := Optional(proposal(1).message),
+        messagesReceived := intermediateState1_2().messagesReceived + {prepare1()}
+    )
+}
+function env1(): Network
+{
+    Network(
+        [0,1,2,3],
+        multiset(outProposal1(1) + outProposal1(2) + outPrepare1()),
+        0,
+        multiset(outProposal1(1) + outProposal1(2) + outPrepare1())
+    )
+}
+function s1(): DSState
+{
+    DSState(
+        config(),
+        env1(),
+        s0().nodes[0 := finalState1()],
+        adv()
+    )
+}
+
+function adv2(): Adversary
+{
+    Adversary({proposal(1).message, proposal(2).message}, {0})
+}
+function newBlock(i: nat): QbftMessageWithRecipient
+{
+    QbftMessageWithRecipient(NewBlock(signedBlock(i)), i)
+}
+function env2(): Network
+{
+    Network([0,1,2,3], multiset{newBlock(1), newBlock(2)}, 0, s1().environment.allMessagesSent + multiset{newBlock(1), newBlock(2)})
+}
+function s2(): DSState
+{
+    s1().(environment := env2(), adversary := adv2())
+}
+
+function newMessagesReceived3(): set<QbftMessage>
+{
+    {newBlock(1).message}
+}
+function currentWithNewMessagesReceived3(): NodeState
+{
+    var current := s2().nodes[1];
+    current.(
+                messagesReceived := newMessagesReceived3(),
+                localTime := current.localTime + 1
+            )
+}
+function intermediateState3_1(): NodeState
+{
+    currentWithNewMessagesReceived3().(
+        blockchain := [genesisBlock(), signedBlock(1)],
+        timeLastRoundStart := 1
+    )
+}
+function proposal3(): QbftMessage
+{
+    var block := getNewBlock(intermediateState3_1(), 0);
+    Proposal(
+        signProposal(
+            UnsignedProposal(
+                2,
+                0,
+                digest(block)),
+            1),
+        block,
+        {},
+        {})
+}
+function outProposal3(): set<QbftMessageWithRecipient>
+{
+    Multicast(
+        [0,1,2,3],
+        proposal3()
+    )
+}
+function intermediateState3_2(): NodeState
+{
+    intermediateState3_1().(
+        messagesReceived := intermediateState3_1().messagesReceived + {proposal3()}
+    )
+}
+function prepare3(): QbftMessage
+{
+    Prepare(
+            signPrepare(
+                UnsignedPrepare(
+                    2,
+                    0,
+                    digest(getNewBlock(intermediateState3_1(), 0))),
+                1
+                )
+        )
+}
+function finalState3(): NodeState
+{
+    intermediateState3_2().(
+        proposalAcceptedForCurrentRound := Optional(proposal3()),
+        messagesReceived := intermediateState3_2().messagesReceived + {prepare3()}
+    )
+}
+function outPrepare3(): set<QbftMessageWithRecipient>
+{
+    Multicast(
+        [0,1,2,3],
+        prepare3()
+    )
+}
+function env3(): Network
+{
+    Network([0,1,2,3], 
+        multiset{newBlock(2)} + multiset(outPrepare3()) + multiset(outProposal3()), 
+        0, 
+        env2().allMessagesSent + multiset(outPrepare3()) + multiset(outProposal3()))
+}
+function s3(): DSState
+{
+    s2().(
+        environment := env3(),
+        nodes := s2().nodes[1 := finalState3()]
+    )
+}
+function newMessagesReceived4(): set<QbftMessage>
+{
+    {newBlock(2).message, proposal3()}
+}
+function currentWithNewMessagesReceived4(): NodeState
+{
+    var current := s3().nodes[2];
+    current.(
+                messagesReceived := newMessagesReceived4(),
+                localTime := current.localTime + 1
+            )
+}
+function intermediateState4(): NodeState
+{
+    currentWithNewMessagesReceived4().(
+        blockchain := [genesisBlock(), signedBlock(2)],
+        timeLastRoundStart := 1
+    )
+}
+function prepare4(): QbftMessage
+{
+    Prepare(
+        signPrepare(
+            UnsignedPrepare(
+                2,
+                0,
+                digest(getNewBlock(intermediateState3_1(), 0))),
+            2
+            )
+        )
+}
+function finalState4(): NodeState
+{
+    intermediateState4().(
+        proposalAcceptedForCurrentRound := Optional(proposal3()),
+        messagesReceived := intermediateState4().messagesReceived + {prepare4()}
+    )
+}
+function outPrepare4(): set<QbftMessageWithRecipient>
+{
+    Multicast(
+        [0,1,2,3],
+        prepare4()
+    )
+}
+
+function env4(): Network
+{
+    Network([0,1,2,3], 
+        env3().messagesSentYetToBeReceived - multiset{newBlock(2), QbftMessageWithRecipient(proposal3(), 2)} + multiset(outPrepare4()),
+        // multiset(outPrepare3()) + multiset{QbftMessageWithRecipient(proposal3(), 0), QbftMessageWithRecipient(proposal3(), 1), QbftMessageWithRecipient(proposal3(), 3)} + multiset(outPrepare4()), 
+        0,
+        env3().allMessagesSent + multiset(outPrepare4()))
+}
+function s4(): DSState
+{
+    s3().(
+        environment := env4(),
+        nodes := s3().nodes[2 := finalState4()]
+    )
+}
 }
